translations

translations/translation_utils.v
@@ -120,12 +120,112 @@ Definition tsl_ident (id : ident) : ident := (id ++ "ᵗ")%string.
 Definition print_nf {A} (msg : A) : TemplateMonad unit
   := (tmEval all msg) >>= tmPrint.
 
+
+Fixpoint extract_mind_decl_from_program (id : ident) (p : program)
+  : option minductive_decl
+  := match p with
+     | PConstr _ _ _ _ p => extract_mind_decl_from_program id p
+     | PType id' n inds p => if string_dec id id' then
+                              Some (Build_minductive_decl n inds)
+                            else extract_mind_decl_from_program id p
+     | PAxiom _ _ _ p => extract_mind_decl_from_program id p
+     | PIn _ => None
+     end.
+
+Fixpoint decompose_prod (t : term) : (list name) * (list term) * term :=
+  match t with
+  | tProd n A B => let (nAs, B) := decompose_prod B in
+                  let (ns, As) := nAs in
+                  (n :: ns, A :: As, B)
+  | _ => ([], [], t)
+  end.
+
+Definition get_ident (n : name) :=
+  match n with
+  | nAnon => "XX"
+  | nNamed i => i
+  end.
+
+Fixpoint remove_arity (n : nat) (t : term) : term :=
+  match n with
+  | O => t
+  | S n => match t with
+          | tProd _ _ B => remove_arity n B
+          | _ => t (* todo *)
+          end
+  end.
+
+Definition option_get {A} (default : A) (x : option A) : A
+  := match x with
+     | Some x => x
+     | None => default
+     end.
+
+Definition mind_decl_to_entry (* (id : ident) *) (decl : minductive_decl)
+  : mutual_inductive_entry.
+Proof.
+  refine ({|
+             mind_entry_record := None; (* not a record *)
+             mind_entry_finite := Finite; (* inductive *)
+             mind_entry_params := _;
+             mind_entry_inds := _;
+             mind_entry_polymorphic := false;
+             mind_entry_private := None;
+           |}).
+  - refine (match List.hd_error decl.(ind_bodies) with
+            | Some i0 => _
+            | None => nil (* todo *)
+            end).
+    pose (typ := decompose_prod i0.(ind_type)).
+    destruct typ as [[names types] _].
+    apply (List.firstn decl.(ind_npars)) in names.
+    apply (List.firstn decl.(ind_npars)) in types.
+    refine (List.combine _ _).
+    exact (List.map get_ident names).
+    exact (List.map LocalAssum types).
+    (* pose (fold_left_i (fun acc i ty => let na := tVar (get_ident (List.nth i names nAnon)) *)
+    (*                                 in (na :: fst acc, substl (fst acc) ty :: snd acc)) types ([], [])). *)
+    (* exact (snd p). *)
+  - refine (List.map _ decl.(ind_bodies)).
+    intros [].
+    refine ({| mind_entry_typename := ind_name;
+               mind_entry_arity := remove_arity decl.(ind_npars) ind_type;
+               mind_entry_template := false;
+               mind_entry_consnames := _;
+               mind_entry_lc := _;
+            |}).
+    
+    refine (List.map (fun x => fst (fst x)) ind_ctors).
+    refine (List.map (fun x => remove_arity decl.(ind_npars)
+                                                (snd (fst x))) ind_ctors).
+Defined.
+
+
+
+
 Definition tTranslate (tsl : Translation) (ΣE : tsl_context) (id : ident)
   : TemplateMonad (option tsl_context) :=
   gr <- tmAbout id ;;
+  id' <- tmEval all (tsl_id id) ;;
   match gr with
-  | IndRef ind
   | ConstructRef ind _ => tmPrint "todo tTranslate" ;; ret None
+  | IndRef (mkInd kn n) =>
+      d <- tmQuoteInductive id ;;
+      let d' := tsl_ind ΣE id d in
+      d' <- tmEval lazy d' ;;
+      (* tmPrint d' ;; *)
+      match d' with
+      | Success (E, decls) =>
+        (* print_nf d' ;; *)
+        let entries := List.map mind_decl_to_entry decls in
+        (* print_nf e ;; *)
+        monad_fold_left (fun _ e => tmMkInductive e) entries tt ;;
+        let decl := InductiveDecl kn d in
+        print_nf  (id ++ " has been translated as " ++ id') ;;
+        ret (Some (decl :: fst ΣE, E ++ snd ΣE)%list)
+      | _ => print_nf "error" ;; ret None
+      end
+
   | ConstRef kn =>
     e <- tmQuoteConstant kn true ;;
     print_nf ("toto1" ++ id) ;;
@@ -146,7 +246,6 @@ Definition tTranslate (tsl : Translation) (ΣE : tsl_context) (id : ident)
         | Error e => tmPrint "tsl error in type: " ;; tmPrint e ;; ret None
         | Success A' =>
           print_nf ("toto4 " ++ id) ;;
-          id' <- tmEval all (tsl_id id) ;;
           tmMkDefinition id' t' ;;
           print_nf ("toto5 " ++ id) ;;
           let decl := {| cst_universes := [];
@@ -218,84 +317,6 @@ Definition tImplementExisting (tsl_id : ident -> ident)
 
 
 
-Fixpoint extract_mind_decl_from_program (id : ident) (p : program)
-  : option minductive_decl
-  := match p with
-     | PConstr _ _ _ _ p => extract_mind_decl_from_program id p
-     | PType id' n inds p => if string_dec id id' then
-                              Some (Build_minductive_decl n inds)
-                            else extract_mind_decl_from_program id p
-     | PAxiom _ _ _ p => extract_mind_decl_from_program id p
-     | PIn _ => None
-     end.
-
-Fixpoint decompose_prod (t : term) : (list name) * (list term) * term :=
-  match t with
-  | tProd n A B => let (nAs, B) := decompose_prod B in
-                  let (ns, As) := nAs in
-                  (n :: ns, A :: As, B)
-  | _ => ([], [], t)
-  end.
-
-Definition get_ident (n : name) :=
-  match n with
-  | nAnon => "XX"
-  | nNamed i => i
-  end.
-
-Fixpoint remove_arity (n : nat) (t : term) : term :=
-  match n with
-  | O => t
-  | S n => match t with
-          | tProd _ _ B => remove_arity n B
-          | _ => t (* todo *)
-          end
-  end.
-
-Definition option_get {A} (default : A) (x : option A) : A
-  := match x with
-     | Some x => x
-     | None => default
-     end.
-
-Definition mind_decl_to_entry (* (id : ident) *) (decl : minductive_decl)
-  : mutual_inductive_entry.
-Proof.
-  refine ({|
-             mind_entry_record := None; (* not a record *)
-             mind_entry_finite := Finite; (* inductive *)
-             mind_entry_params := _;
-             mind_entry_inds := _;
-             mind_entry_polymorphic := false;
-             mind_entry_private := None;
-           |}).
-  - refine (match List.hd_error decl.(ind_bodies) with
-            | Some i0 => _
-            | None => nil (* todo *)
-            end).
-    pose (typ := decompose_prod i0.(ind_type)).
-    destruct typ as [[names types] _].
-    apply (List.firstn decl.(ind_npars)) in names.
-    apply (List.firstn decl.(ind_npars)) in types.
-    refine (List.rev (List.combine _ _)).
-    exact (List.map get_ident names).
-    exact (List.map LocalAssum types).
-    (* pose (fold_left_i (fun acc i ty => let na := tVar (get_ident (List.nth i names nAnon)) *)
-    (*                                 in (na :: fst acc, substl (fst acc) ty :: snd acc)) types ([], [])). *)
-    (* exact (snd p). *)
-  - refine (List.map _ decl.(ind_bodies)).
-    intros [].
-    refine ({| mind_entry_typename := ind_name;
-               mind_entry_arity := remove_arity decl.(ind_npars) ind_type;
-               mind_entry_template := false;
-               mind_entry_consnames := _;
-               mind_entry_lc := _;
-            |}).
-    
-    refine (List.map (fun x => fst (fst x)) ind_ctors).
-    refine (List.map (fun x => remove_arity decl.(ind_npars)
-                                                (snd (fst x))) ind_ctors).
-Defined.
 
 (* Inductive eq' (A : Set) (x : A) : A -> Prop :=  eq_refl' : eq' A x x. *)
 (* Quote Recursively Definition eq'_prog := eq'. *)
@@ -309,7 +330,7 @@ Quote Recursively Definition nat_prog := nat.
 Definition eq_decl := Eval compute in
       option_get todo (extract_mind_decl_from_program "Coq.Init.Logic.eq" eq_prog).
 Definition sigma_decl := Eval compute in
-      option_get todo (extract_mind_decl_from_program "Template.sigma.sigma" sigma_prog).
+      option_get todo (extract_mind_decl_from_program "Translations.sigma.sigma" sigma_prog).
 Definition nat_decl := Eval compute in
       option_get todo (extract_mind_decl_from_program "Coq.Init.Datatypes.nat" nat_prog).
 
