translations/tsl_param3.v
@@ -10,24 +10,20 @@ Open Scope string_scope.
 Open Scope sigma_scope.
 
 
-
-
-Reserved Notation "'tsl_ty_param'".
-
-
 Definition tsl_name n :=
   match n with
   | nAnon => nAnon
   | nNamed n => nNamed (tsl_ident n)
   end.
 
-(* Definition mkApps t us := *)
-(*   match t with *)
-(*   | tApp f args => tApp f (args ++ us) *)
-(*   | _ => tApp t us *)
-(*   end. *)
-Definition mkApps t us := tApp t us. (* meanwhile *)
+Definition mkApps t us :=
+  match t with
+  | tApp f args => tApp f (args ++ us)
+  | _ => tApp t us
+  end.
+(* Definition mkApps t us := tApp t us. (* meanwhile *) *)
 
+Definition mkApp t u := mkApps t [u].
 
 Fixpoint subst_app (t : term) (us : list term) : term :=
   match t, us with
@@ -37,15 +33,16 @@ Fixpoint subst_app (t : term) (us : list term) : term :=
   end.
 
 
+Definition default_term := tVar "constant not found".
 
 Fixpoint tsl_rec0 (n : nat) (t : term) {struct t} : term :=
   match t with
   | tRel k => if k >= n then tRel (2*k+1) else t
   | tEvar k ts => tEvar k (map (tsl_rec0 n) ts)
   | tCast t c a => tCast (tsl_rec0 n t) c (tsl_rec0 n a)
-  | tProd x A B => tProd x (tsl_rec0 n A) (tsl_rec0 (n+1) B)
-  | tLambda x A t => tLambda x (tsl_rec0 n A) (tsl_rec0 (n+1) t)
-  | tLetIn x a t u => tLetIn x (tsl_rec0 n a) (tsl_rec0 n t) (tsl_rec0 (n+1) u)
+  | tProd na A B => tProd na (tsl_rec0 n A) (tsl_rec0 (n+1) B)
+  | tLambda na A t => tLambda na (tsl_rec0 n A) (tsl_rec0 (n+1) t)
+  | tLetIn na a t u => tLetIn na (tsl_rec0 n a) (tsl_rec0 n t) (tsl_rec0 (n+1) u)
   | tApp t lu => tApp (tsl_rec0 n t) (map (tsl_rec0 n) lu)
   | tCase ik t u br => tCase ik (tsl_rec0 n t) (tsl_rec0 n u)
                             (map (fun x => (fst x, tsl_rec0 n (snd x))) br)
@@ -55,41 +52,40 @@ Fixpoint tsl_rec0 (n : nat) (t : term) {struct t} : term :=
   | _ => t
   end.
 
-Definition default_term := tRel 0.    
-
-Fixpoint tsl_rec1 (E : tsl_table) (n : nat) (t : term) : term :=
+Fixpoint tsl_rec1 (E : tsl_table) (t : term) : term :=
   match t with
   | tRel k => tRel (2 * k)
   | tSort s => tLambda (nNamed "A") (tSort s) (tProd nAnon (tRel 0) (tSort s))
 
-  | tProd na A B => let ΠAB0 := tsl_rec0 n (tProd na A B) in
-                  let A0 := tsl_rec0 n A in
-                  let A1 := tsl_rec1 E n A in
-                  let B1 := tsl_rec1 E n B in
-                  tLambda (nNamed "f") ΠAB0
-                               (tProd na (lift0 1 A0) (tProd (tsl_name na) (subst_app (lift0 2 A1) [tRel 0])
+  | tProd na A B => let A0 := tsl_rec0 0 A in
+                   let A1 := tsl_rec1 E A in
+                   let B0 := tsl_rec0 1 B in
+                   let B1 := tsl_rec1 E B in
+                   let ΠAB0 := tProd na A0 B0 in
+                   tLambda (nNamed "f") ΠAB0
+                           (tProd na (lift0 1 A0) (tProd (tsl_name na) (subst_app (lift0 2 A1) [tRel 0])
                                       (subst_app (lift 1 2 B1)
                                             [tApp (tRel 2) [tRel 1]])))
 
-  | tLambda na A t => let A0 := tsl_rec0 n A in
-                    let A1 := tsl_rec1 E n A in
-                    tLambda na A0 (tLambda (tsl_name na) (subst_app (lift0 1 A1) [tRel 0]) (tsl_rec1 E n t))
+  | tLambda na A t => let A0 := tsl_rec0 0 A in
+                     let A1 := tsl_rec1 E A in
+                     tLambda na A0 (tLambda (tsl_name na) (subst_app (lift0 1 A1) [tRel 0]) (tsl_rec1 E t))
 
-  | tApp t u => let u' := List.fold_left (fun l v => tsl_rec0 n v :: tsl_rec1 E n v :: l) u [] in
-               mkApps (tsl_rec1 E n t) u'
+  | tApp t us => let us' := flatten (map (fun v => [tsl_rec0 0 v; tsl_rec1 E v]) us) in
+                mkApps (tsl_rec1 E t) us'
 
-  | tLetIn na t A u => let t0 := tsl_rec0 n t in
-                     let t1 := tsl_rec1 E n t in
-                     let A0 := tsl_rec0 n A in
-                     let A1 := tsl_rec1 E n A in
-                     let u0 := tsl_rec0 n u in
-                     let u1 := tsl_rec1 E n u in
-                     tLetIn na t0 A0 (tLetIn (tsl_name na) (lift0 1 t1) (subst_app (lift0 1 A1) [tRel 0]) u1)
+  | tLetIn na t A u => let t0 := tsl_rec0 0 t in
+                      let t1 := tsl_rec1 E t in
+                      let A0 := tsl_rec0 0 A in
+                      let A1 := tsl_rec1 E A in
+                      let u0 := tsl_rec0 0 u in
+                      let u1 := tsl_rec1 E u in
+                      tLetIn na t0 A0 (tLetIn (tsl_name na) (lift0 1 t1) (subst_app (lift0 1 A1) [tRel 0]) u1)
 
-  | tCast t c A => let t0 := tsl_rec0 n t in
-                  let t1 := tsl_rec1 E n t in
-                  let A0 := tsl_rec0 n A in
-                  let A1 := tsl_rec1 E n A in
+  | tCast t c A => let t0 := tsl_rec0 0 t in
+                  let t1 := tsl_rec1 E t in
+                  let A0 := tsl_rec0 0 A in
+                  let A1 := tsl_rec1 E A in
                   tCast t1 c (mkApps A1 [tCast t0 c A0]) (* apply_subst ? *)
 
   | tConst s univs =>
@@ -141,17 +137,8 @@ Definition map_i {A B} f := @map_i_aux A B f 0.
 
 
 Definition tsl_mind_decl (E : tsl_table)
-           (id : ident) (mind : minductive_decl)
-  : tsl_table * list minductive_decl.
-  refine (_, [{| ind_npars := 2 * mind.(ind_npars);
-                 ind_bodies := _ |}]).
-  - refine (let id' := tsl_ident id in (* should be kn ? *)
-            fold_left_i (fun E i ind => _ :: _ ++ E)%list mind.(ind_bodies) []).
-    + (* ind *)
-      exact (IndRef (mkInd id i), tInd (mkInd id' i) []).
-    + (* ctors *)
-      refine (fold_left_i (fun E k _ => _ :: E) ind.(ind_ctors) []).
-      exact (ConstructRef (mkInd id i) k, tConstruct (mkInd id' i) k []).
+           (kn : kername) (mind : minductive_decl) : minductive_decl.
+  refine {| ind_npars := 2 * mind.(ind_npars); ind_bodies := _ |}.
   - refine (map_i _ mind.(ind_bodies)).
     intros i ind.
     refine {| ind_name := tsl_ident ind.(ind_name);
@@ -160,20 +147,29 @@ Definition tsl_mind_decl (E : tsl_table)
               ind_ctors := _;
               ind_projs := [] |}. (* todo *)
     + (* arity  *)
-      refine (let ar := subst_app (tsl_rec1 E 0 ind.(ind_type))
-                             [tInd (mkInd id i) []] in
+      refine (let ar := subst_app (tsl_rec1 E ind.(ind_type))
+                                  [tInd (mkInd kn i) []] in
               ar).
     + (* constructors *)
       refine (map_i _ ind.(ind_ctors)).
       intros k ((name, typ), nargs).
       refine (tsl_ident name, _, 2 * nargs).
-      refine (subst_app _ [tConstruct (mkInd id i) k []]).
-      refine (fold_left_i (fun t0 i u  => t0 {S i := u}) _ (tsl_rec1 E 0 typ)).
+      refine (subst_app _ [tConstruct (mkInd kn i) k []]).
+      refine (fold_left_i (fun t0 i u  => t0 {S i := u}) _ (tsl_rec1 E typ)).
       (* [I_n-1; ... I_0] *)
-      refine (List.rev (map_i (fun i _ => tInd (mkInd id i) [])
+      refine (List.rev (map_i (fun i _ => tInd (mkInd kn i) [])
                               mind.(ind_bodies))).
 Defined.
 
+Definition tsl_ind_extend_table (kn kn' : kername) (mind : minductive_decl)
+  : tsl_table.
+  refine (fold_left_i (fun E i ind => _ :: _ ++ E)%list mind.(ind_bodies) []).
+  + (* ind *)
+    exact (IndRef (mkInd kn i), tInd (mkInd kn' i) []).
+  + (* ctors *)
+    refine (fold_left_i (fun E k _ => _ :: E) ind.(ind_ctors) []).
+    exact (ConstructRef (mkInd kn i) k, tConstruct (mkInd kn' i) k []).
+Defined.
 
 (* Instance param3 : Translation *)
 (*   := {| tsl_id := tsl_ident ; *)
@@ -183,11 +179,11 @@ Defined.
 
 
 Run TemplateProgram (tm <- tmQuote (forall A, A -> A) ;;
-                     let tm' := tsl_rec1 [] 0 tm in
+                     let tm' := tsl_rec1 [] tm in
                      tmUnquote tm' >>= tmPrint).
 
 Run TemplateProgram (tm <- tmQuote (fun A (x : A) => x) ;;
-                     let tm' := tsl_rec1 [] 0 tm in
+                     let tm' := tsl_rec1 [] tm in
                      tmUnquote tm' >>= tmPrint).
 
 Goal ((fun f : forall A : Type, A -> A =>
@@ -199,399 +195,67 @@ Defined.
 Quote Definition tm := ((fun A (x:A) => x) (Type -> Type) (fun x => x)).
 
 Run TemplateProgram (
-                     let tm' := tsl_rec1 [] 0 tm in
+                     let tm' := tsl_rec1 [] tm in
                      print_nf tm' ;;
                      tmUnquote tm' >>= tmPrint).
 
 
 
 Definition tTranslate (ΣE : tsl_context) (id : ident)
-  : TemplateMonad (option tsl_context) :=
+  : TemplateMonad (tsl_context) :=
   gr <- tmAbout id ;;
   id' <- tmEval all (tsl_ident id) ;;
+  let Σ := fst ΣE in
   let E := snd ΣE in
   match gr with
-  | ConstructRef ind _ => tmPrint "todo tTranslate" ;; ret None
+  | ConstructRef ind _ => tmPrint "todo tTranslate" ;; ret ΣE
   | IndRef (mkInd kn n) =>
       d <- tmQuoteInductive id ;;
-      let d' := tsl_mind_decl E id d in
-      d' <- tmEval lazy d' ;;
-      tmPrint d' ;;
-      let entries := map mind_decl_to_entry (snd d') in
-      (* print_nf entries ;; *)
-      monad_fold_left (fun _ e => tmMkInductive e) entries tt ;;
-      let decl := InductiveDecl kn d in
-      print_nf  (id ++ " has been translated as " ++ id') ;;
-      ret (Some (decl :: fst ΣE, E ++ snd ΣE)%list)
+      let e' := mind_decl_to_entry (tsl_mind_decl E kn d) in
+      e' <- tmEval lazy e' ;;
+      tmPrint e' ;;
+      tmMkInductive e' ;;
+      gr' <- tmAbout id' ;;
+      match gr' with
+      | IndRef (mkInd kn' _) =>
+        let E' := tsl_ind_extend_table kn kn' d in
+        print_nf  (id ++ " has been translated as " ++ id') ;;
+        ret (InductiveDecl kn d :: Σ, E' ++ E)%list
+      | _ => tmPrint gr' ;; tmPrint "not found" ;; ret ΣE
+      end
 
   | ConstRef kn =>
     e <- tmQuoteConstant kn true ;;
     print_nf ("toto1" ++ id) ;;
     match e with
     | ParameterEntry _ => print_nf (id ++ "is an axiom, not a definition") ;;
-                         ret None
+                         ret ΣE
     | DefinitionEntry {| definition_entry_type := A;
                          definition_entry_body := t |} =>
       print_nf ("toto2 " ++ id) ;;
-      (* tmPrint t ;; *)
       t0 <- tmEval lazy (tsl_rec0 0 t) ;;
-      t1 <- tmEval lazy (tsl_rec1 E 0 t) ;;
-      A1 <- tmEval lazy (tsl_rec1 E 0 A) ;;
+      t1 <- tmEval lazy (tsl_rec1 E t) ;;
+      A1 <- tmEval lazy (tsl_rec1 E A) ;;
       print_nf ("toto4 " ++ id) ;;
+      print_nf t1 ;;
       tmMkDefinition id' t1 ;;
       print_nf ("toto5 " ++ id) ;;
       let decl := {| cst_universes := [];
                      cst_type := A; cst_body := Some t |} in
-      let Σ' := ConstantDecl kn decl :: (fst ΣE) in
-      let E' := (ConstRef kn, tConst id' []) :: (snd ΣE) in
       print_nf  (id ++ " has been translated as " ++ id') ;;
-      tmEval all (Some (Σ', E'))
+      ret (ConstantDecl kn decl :: Σ, (ConstRef kn, tConst id' []) :: E)
     end
   end.
 
 
-(* Run TemplateProgram (ΣE <- tTranslate ([],[]) "nat" ;; *)
-(*                      let ΣE := option_get todo ΣE in *)
-(*                         (* print_nf ΣE). *) *)
-(*                      tTranslate ΣE "t" >>= tmPrint). *)
-
-Run TemplateProgram (tTranslate ([],[]) "list").
-
-
-
-Definition option_get {A} (default : A) (x : option A) : A
-  := match x with
-     | Some x => x
-     | None => default
-     end.
-
-Definition map_context_decl (f : term -> term) (decl : context_decl): context_decl
-  := {| decl_name := decl.(decl_name);
-        decl_body := option_map f decl.(decl_body); decl_type := f decl.(decl_type) |}.
-
-
-Notation " Γ ,, d " := (d :: Γ) (at level 20, d at next level, only parsing).
-  
-Fixpoint tsl_ctx (E : tsl_table) (Γ : context) : context :=
-  match Γ with
-  | [] => []
-  (* | Γ ,, {| decl_name := n; decl_body := None; decl_type := A |} => *)
-  (*   tsl_ctx E Γ ,, vass n (tsl_rec0 0 A) ,, vass (tsl_name n) (mkApp (lift0 1 (tsl_rec1 E 0 A)) (tRel 0)) *)
-  | Γ ,, decl => let n := decl.(decl_name) in
-                let x := decl.(decl_body) in
-                let A := decl.(decl_type) in
-    tsl_ctx E Γ ,, Build_context_decl n (omap (tsl_rec0 0) x) (tsl_rec0 0 A) 
-                ,, Build_context_decl (tsl_name n) (omap (lift 1 0 \o tsl_rec1 E 0) x) (mkApps (lift0 1 (tsl_rec1 E 0 A)) [tRel 0])
-  end.
-
-Delimit Scope term_scope with term.
-
-Notation "#| Γ |" := (List.length Γ) (at level 0, Γ at level 99, format "#| Γ |") : term_scope.
-
-  
-Lemma tsl_ctx_length E (Γ : context) : #|tsl_ctx E Γ| = 2 * #|Γ|%term.
-Proof.
-  induction Γ.
-  reflexivity.
-  destruct a, decl_body; simpl;
-  by rewrite IHΓ mulnS.
-Qed.
-
-(* Fixpoint removefirst_n {A} (n : nat) (l : list A) : list A := *)
-(*   match n with *)
-(*   | O => l *)
-(*   | S n => match l with *)
-(*           | [] => [] *)
-(*           | a :: l => removefirst_n n l *)
-(*           end *)
-(*   end. *)
-
-Notation "( x ; y )" := (exist _ x y).
-
-(* Lemma tsl_ctx_safe_nth fuel Σ E Γ *)
-(*   : forall Γ', tsl_ctx fuel Σ E Γ = Success Γ' -> forall n p, exists p', *)
-(*         map_context_decl (tsl_ty fuel Σ E (removefirst_n (S n) Γ)) *)
-(*                          (safe_nth Γ (n; p)) *)
-(*         = Success (safe_nth Γ' (n; p')). *)
-(*   intros Γ' H n p. cbn beta in *. *)
-(*   revert Γ Γ' H p. *)
-(*   induction n; intros Γ Γ' H p; *)
-(*     (destruct Γ as [|A Γ]; [inversion p|]). *)
-(*   - cbn -[map_context_decl]. *)
-(*     rewrite tsl_ctx_cons in H. *)
-(*     remember (map_context_decl (tsl_term fuel Σ E Γ) A).  *)
-(*     destruct t; [|discriminate]. *)
-(*     remember (tsl_ctx fuel Σ E Γ).  *)
-(*     destruct t; [|discriminate]. *)
-(*     cbn in H. inversion H; clear H. *)
-(*     clear p H1. *)
-(*     unshelve econstructor. apply le_n_S, le_0_n. *)
-(*     reflexivity. *)
-(*   - cbn -[map_context_decl]. *)
-(*     rewrite tsl_ctx_cons in H. *)
-(*     remember (map_context_decl (tsl_term fuel Σ E Γ) A).  *)
-(*     destruct t; [|discriminate]. *)
-(*     remember (tsl_ctx fuel Σ E Γ).  *)
-(*     destruct t; [|discriminate]. *)
-(*     cbn in H. inversion H; clear H. *)
-(*     symmetry in Heqt0. *)
-(*     set (Typing.safe_nth_obligation_2 context_decl (A :: Γ) (S n; p) A Γ eq_refl n eq_refl). *)
-(*     specialize (IHn Γ c0 Heqt0 l). *)
-(*     destruct IHn. *)
-    
-(*     unshelve econstructor. *)
-(*     cbn. rewrite <- (tsl_ctx_length fuel Σ E Γ _ Heqt0). exact p. *)
-(*     etransitivity. exact π2. cbn. *)
-(*     apply f_equal, f_equal, f_equal. *)
-(*     apply le_irr. *)
-(* Defined. *)
-(* Admitted. *)
-
-(* (* todo inductives *) *)
-(* Definition global_ctx_correct (Σ : global_context) (E : tsl_context) *)
-(*   := forall id T, lookup_constant_type Σ id = Checked T *)
-(*                 -> exists fuel t' T', lookup_tsl_ctx E (ConstRef id) = Some t' /\ *)
-(*                            tsl_term fuel Σ E [] T = Success _ T' /\ *)
-(*                            squash (Σ ;;; [] |-- t' : T'). *)
-
-
-Definition tsl_table_correct (Σ : global_context) (E : tsl_table) : Type := todo.
-(*   := forall id t' T, *)
-(*     lookup_tsl_table E (ConstRef id) = Some t' -> *)
-(*     lookup_constant_type Σ id = Checked T -> *)
-(*     exists fuel T', ((tsl_ty fuel Σ E [] T = Success T') *)
-(*       * (Σ ;;; [] |--  t' : T'))%type. *)
-
-Lemma LmapE : @List.map = @seq.map.
-reflexivity.
-Qed.
-
-Lemma lebE (m n : nat) : (Nat.leb m n) = (m <= n).
-Admitted.
-
-Lemma term_eqP : Equality.axiom eq_term.
-Admitted.
-
-Definition term_eqMixin := EqMixin term_eqP.
-Canonical termT_eqype := EqType term term_eqMixin.
-
-Lemma tsl_rec0_lift m n t :
-  tsl_rec0 m (lift n m t) = lift (2 * n) m (tsl_rec0 m t).
-Proof.
-elim/term_forall_list_ind : t m n => //=; rewrite ?plusE.
-- move=> n m k.
-  rewrite lebE.
-  case: leqP => /= mn; rewrite lebE plusE.
-  rewrite !ifT ?mulnDr ?addnA //.
-    admit.
-    admit.
-  by rewrite leqNgt mn.
-- admit.
-- by move=> t IHt c t0 IHt0 m n; rewrite IHt IHt0.
-- by move=> n0 t -IHt t0 IHt0 m n /=; rewrite IHt addn1 IHt0.
-- by move=> n t IHt t0 IHt0 m n0; rewrite IHt addn1 IHt0.
-- by move=> n t IHt t0 IHt0 t1 IHt1 m n0; rewrite !addn1 IHt IHt0 IHt1.
-- move=> t IHt l IHl m n; rewrite IHt.
-  rewrite LmapE.
-  rewrite -!map_comp.
-  congr (tApp _ _).
-  apply/eq_in_map => i /=.
-  admit.
-- move=> p t IHt t0 IHt0 l IHl m n.
-  rewrite IHt IHt0.
-  admit.
-- by move=> s t IHt m n; rewrite IHt.
-- admit.
-- admit.
-Admitted.
-
-
-Lemma lift_mkApps n k t us
-  : lift n k (mkApps t us) = mkApps (lift n k t) (map (lift n k) us).
-Proof.
-  (* destruct t; try reflexivity. *)
-  (* cbn. destruct (Nat.leb k n0); try reflexivity. *)
-  (* cbn. by rewrite -map_cat.  *)
-done.
-Qed.
-
-Arguments subst_app : simpl nomatch.
-
-Lemma tsl_rec1_lift E n t :
-  (* tsl_rec1 E 0 (lift n m t) = lift (2 * n) (2 * m) (tsl_rec1 E 0 t). *)
-  tsl_rec1 E 0 (lift0 n t) = lift0 (2 * n) (tsl_rec1 E 0 t).
-Proof.
-elim/term_forall_list_ind : t n => //; rewrite ?plusE.
-- move=> n k.
-  (* rewrite !lebE fun_if /= leq_mul2l /=. *)
-  (* by have [] := leqP m n => //=; *) by rewrite /= mulnDr.
-- admit.
-- admit.
-- admit.
-- move=> t IHt c t0 IHt0 n /=; rewrite IHt IHt0 ?lift_mkApps.
-  congr (tCast _ _ (mkApps _ _)).
-  by rewrite !tsl_rec0_lift.
-- move=> n t IHt t0 IHt0 n0.
-  rewrite /=.
-  rewrite !IHt.
-  rewrite !tsl_rec0_lift.
-(*   rewrite lift_simpl. *)
-(*   rewrite IHt addn1 IHt0. *)
-(* - by move=> n t IHt t0 IHt0 m n0; rewrite IHt addn1 IHt0. *)
-(* - by move=> n t IHt t0 IHt0 t1 IHt1 m n0; rewrite !addn1 IHt IHt0 IHt1. *)
-(* - move=> t IHt l IHl m n; rewrite IHt. *)
-(*   rewrite LmapE. *)
-(*   rewrite -!map_comp. *)
-(*   congr (tApp _ _). *)
-(*   apply/eq_in_map => i /=. *)
-(*   admit. *)
-(* - move=> p t IHt t0 IHt0 l IHl m n. *)
-(*   rewrite IHt IHt0. *)
-(*   admit. *)
-(* - by move=> s t IHt m n; rewrite IHt. *)
-(* - admit. *)
-(* - admit. *)
-Admitted.
-
-  
-
-
-
-(* Admitted. *)
-
-(* Lemma tsl_rec0_lift n t *)
-(*   : tsl_rec0 0 (lift0 n t) = lift0 n (tsl_rec0 0 t). *)
-(* Admitted. *)
-
-(* Lemma tsl_ty_lift fuel Σ E Γ n (p : n <= #|Γ|) t *)
-(*   : tsl_ty fuel Σ E Γ (lift0 n t) = *)
-(*     (t' <- tsl_ty fuel Σ E (removefirst_n n Γ) t ;; ret (lift0 n t')). *)
-(* Admitted. *)
-
-(* Lemma tsl_S_fuel {fuel Σ E Γ t t'} *)
-(*   : tsl_term fuel Σ E Γ t = Success t' -> tsl_term (S fuel) Σ E Γ t = Success t'. *)
-(* Admitted. *)
-
-
-Record hidden T := Hidden {show : T}.
-Arguments show : simpl never.
-Notation "'hidden" := (show _ (Hidden _ _)).
-Lemma hide T (t : T) : t = show T (Hidden T t).
-Proof. by []. Qed.
-
-(* From mathcomp Require Import ssrnat. *)
-
-Arguments safe_nth : simpl nomatch.
-    
-Lemma eq_safe_nth T (l : list T) n n' p p' : n = n' ->
-  safe_nth l (n; p) = safe_nth l (n'; p') :> T. 
-Proof.
-move=> eq_n; case: _ / eq_n in p p' *.
-elim: l => [|x l IHl] in n p p' *.
-  by inversion p.
-by case: n => [//|n] in p p' *; apply: IHl.
-Qed.
-
-    Lemma tsl_rec0_decl_type (Γ : context) (n : nat) (isdecl : (n < #|Γ|%term)%coq_nat) (E : tsl_table) (isdecl' : (2 * n + 1 < #|tsl_ctx E Γ|%term)%coq_nat)
-      : tsl_rec0 0 (decl_type (safe_nth Γ (n; isdecl))) =
-        decl_type (safe_nth (tsl_ctx E Γ) (2 * n + 1; isdecl')).
-    Proof.
-      elim: Γ => [|a Γ IHΓ] in n isdecl isdecl' *.
-        by inversion isdecl.
-      simpl.
-      case: n => [//|n] in isdecl isdecl' *.
-      rewrite addn1 /= in isdecl' *.
-      rewrite IHΓ addn1 //.
-        apply/leP; move/leP : isdecl'.
-        by rewrite !mul2n doubleS.
-      move=> isdecl''.
-      congr (decl_type _); apply: eq_safe_nth.
-      by rewrite plusE addn0 mul2n -addnn addnS.
-    Qed.
-
-
-Lemma tsl_rec1_decl_type (Γ : context) (n : nat) (E : tsl_table) p p'
-  (Γ' := tsl_ctx E Γ) :
-  mkApps (lift0 1 (decl_type (safe_nth Γ' ((2 * n); p)))) [tRel 0] = 
-  decl_type (safe_nth Γ' (2 * n; p')).
-Proof.
-subst Γ'; elim: Γ => [|a Γ IHΓ] in n p p' *.
-  by inversion p.
-(* simpl. *)
-(* case: n => [|n] //= in p p' *. *)
-
-(* rewrite /=. *)
-(* rewrite addn1 /= in p' *. *)
-(* rewrite IHΓ addn1 //. *)
-(*   apply/leP; move/leP : p'. *)
-(*   by rewrite !mul2n doubleS. *)
-(* move=> p''. *)
-(* congr (decl_type _); apply: eq_safe_nth. *)
-(* by rewrite plusE addn0 mul2n -addnn addnS. *)
-(*     Qed. *)
-
-
-Admitted.
-
-    (* Lemma tsl_rec1_decl_type (Γ : context) (n : nat) (isdecl : (n < #|Γ|%term)%coq_nat) (E : tsl_table) (isdecl' : (2 * n + 1 < #|tsl_ctx E Γ|%term)%coq_nat) *)
-    (*   : tsl_rec1 E (decl_type (safe_nth Γ (n; isdecl))) = *)
-    (*     decl_type (safe_nth (tsl_ctx E Γ) (2 * n + 1; isdecl')). *)
-   
-Lemma tsl_correct Σ Γ t T (H : Σ ;;; Γ |-- t : T)
-  : forall E, tsl_table_correct Σ E ->
-    let Γ' := tsl_ctx E Γ in
-    let t0 := tsl_rec0 0 t in
-    let t1 := tsl_rec1 E 0 t in
-    let T0 := tsl_rec0 0 T in
-    let T1 := tsl_rec1 E 0 T in
-    Σ ;;; Γ' |-- t0 : T0 /\ Σ ;;; Γ' |-- t1 : mkApps T1 [t0].
-Proof.
-elim/typing_ind: H => {Γ t T} Γ.
-- move=> n isdecl E X Γ' /=.
-  rewrite tsl_rec0_lift mulnS add2n (tsl_rec0_decl_type _ _ _ E).
-  rewrite tsl_ctx_length.
-     apply/leP.
-       by rewrite addn1 mul2n -doubleS -mul2n leq_mul2l; apply/leP.
-  rewrite !addn1; move=> isdecl'.
-  split; first exact: type_Rel.
-  have := type_Rel Σ Γ' (2 * n) _.
-
-  evar (l : (2 * n < #|Γ'|%term)%coq_nat).
-  move=> /(_ l).
-  rewrite -tsl_rec1_decl_type /=.
-  admit.
-  (* rewrite simpl_lift_rec; do ?easy. *)
-  (* by rewrite plusE addn0 addn1. *)
-
-
-  
-
-- admit.
-- admit.
-- admit.
-- admit.
-- admit.
-- rewrite /= => t l t' t'' tt' IHt' spine E ΣE_correct; rewrite /mkApps; split.
-    apply: type_App.
-      have [] := IHt' _ ΣE_correct.
-        by move=> t0_ty ?; exact: t0_ty.
-    admit.
-  apply: type_App.
-    have [] := IHt' _ ΣE_correct.
-    by move=> ? t1_ty; exact: t1_ty.
-  admit.
-   
-
-    
-  
-
-
-    rewrite /Γ' => isdecl'; clear.
-    case: Γ isdecl isdecl'.
-    
-    
-      
+(* Definition map_type := forall A B, (A -> B) -> list A -> list B. *)
+(* Definition rev_type := forall A, list A -> list A. *)
+(* Run TemplateProgram (TC <- tTranslate ([],[]) "list" ;; *)
+(*                      TC <- tTranslate TC "rev_type" ;; *)
+(*                      tmDefinition "TC" TC ). *)
 
 
 Require Import Vector.
-(* Run TemplateProgram (ΣE <- tTranslate ([],[]) "nat" ;; *)
+Run TemplateProgram (ΣE <- tTranslate ([],[]) "nat" ;;
+                        (* print_nf ΣE). *)
+                     tTranslate ΣE "t" >>= tmPrint).
